tests/lean/run/matchGenEqns.lean
@@ -20,7 +20,7 @@ info: myTest.match_1.splitter.{u_1, u_2} {α : Type u_1} (motive : List α → S
 #guard_msgs in
 #check myTest.match_1.splitter
 /--
-info: myTest.match_1.gen_eq_1.{u_1, u_2} {α : Type u_1} (motive : List α → Sort u_2) (x✝ : List α)
+info: myTest.match_1.congr_eq_1.{u_1, u_2} {α : Type u_1} (motive : List α → Sort u_2) (x✝ : List α)
   (h_1 : (a : α) → (dc : List α) → x✝ = a :: dc → motive (a :: dc)) (h_2 : (x' : List α) → x✝ = x' → motive x') (a : α)
   (dc : List α) (heq_1 : x✝ = a :: dc) :
   HEq
@@ -30,10 +30,10 @@ info: myTest.match_1.gen_eq_1.{u_1, u_2} {α : Type u_1} (motive : List α → S
     (h_1 a dc heq_1)
 -/
 #guard_msgs in
-#check myTest.match_1.gen_eq_1
+#check myTest.match_1.congr_eq_1
 
 /--
-info: myTest.match_1.gen_eq_2.{u_1, u_2} {α : Type u_1} (motive : List α → Sort u_2) (x✝ : List α)
+info: myTest.match_1.congr_eq_2.{u_1, u_2} {α : Type u_1} (motive : List α → Sort u_2) (x✝ : List α)
   (h_1 : (a : α) → (dc : List α) → x✝ = a :: dc → motive (a :: dc)) (h_2 : (x' : List α) → x✝ = x' → motive x')
   (x' : List α) (heq_1 : x✝ = x') :
   (∀ (a : α) (dc : List α), x' = a :: dc → False) →
@@ -44,7 +44,7 @@ info: myTest.match_1.gen_eq_2.{u_1, u_2} {α : Type u_1} (motive : List α → S
       (h_2 x' heq_1)
 -/
 #guard_msgs in
-#check myTest.match_1.gen_eq_2
+#check myTest.match_1.congr_eq_2
 
 
 def take (n : Nat) (xs : List α) : List α := match n, xs with
@@ -61,7 +61,7 @@ info: take.match_1.{u_1, u_2} {α : Type u_1} (motive : Nat → List α → Sort
 #check take.match_1
 
 /--
-info: take.match_1.gen_eq_1.{u_1, u_2} {α : Type u_1} (motive : Nat → List α → Sort u_2) (n✝ : Nat) (xs✝ : List α)
+info: take.match_1.congr_eq_1.{u_1, u_2} {α : Type u_1} (motive : Nat → List α → Sort u_2) (n✝ : Nat) (xs✝ : List α)
   (h_1 : (x : List α) → motive 0 x) (h_2 : (n : Nat) → motive n.succ [])
   (h_3 : (n : Nat) → (a : α) → (as : List α) → motive n.succ (a :: as)) (x✝ : List α) (heq_1 : n✝ = 0)
   (heq_2 : xs✝ = x✝) :
@@ -72,7 +72,7 @@ info: take.match_1.gen_eq_1.{u_1, u_2} {α : Type u_1} (motive : Nat → List α
     | n.succ, a :: as => h_3 n a as)
     (h_1 x✝)
 -/
-#guard_msgs in #check take.match_1.gen_eq_1
+#guard_msgs in #check take.match_1.congr_eq_1
 
 def matchOptionUnit (o? : Option Unit) : Bool := Id.run do
     if let some _ := o? then
@@ -81,7 +81,7 @@ def matchOptionUnit (o? : Option Unit) : Bool := Id.run do
       false
 
 /--
-info: matchOptionUnit.match_1.gen_eq_1.{u_1} (motive : Option Unit → Sort u_1) (o?✝ : Option Unit)
+info: matchOptionUnit.match_1.congr_eq_1.{u_1} (motive : Option Unit → Sort u_1) (o?✝ : Option Unit)
   (h_1 : (val : Unit) → motive (some val)) (h_2 : (x : Option Unit) → motive x) (val✝ : Unit)
   (heq_1 : o?✝ = some val✝) :
   HEq
@@ -91,7 +91,7 @@ info: matchOptionUnit.match_1.gen_eq_1.{u_1} (motive : Option Unit → Sort u_1)
     (h_1 val✝)
 -/
 #guard_msgs in
-#check matchOptionUnit.match_1.gen_eq_1
+#check matchOptionUnit.match_1.congr_eq_1
 
 set_option linter.unusedVariables false in
 partial def utf16PosToCodepointPosFromAux (s : String) : Nat → String.Pos → Nat → Bool
@@ -99,7 +99,7 @@ partial def utf16PosToCodepointPosFromAux (s : String) : Nat → String.Pos → 
   | utf16pos, utf8pos, cp => false
 
 /--
-info: utf16PosToCodepointPosFromAux.match_1.gen_eq_1.{u_1} (motive : Nat → String.Pos → Nat → Sort u_1) (x✝ : Nat)
+info: utf16PosToCodepointPosFromAux.match_1.congr_eq_1.{u_1} (motive : Nat → String.Pos → Nat → Sort u_1) (x✝ : Nat)
   (x✝¹ : String.Pos) (x✝² : Nat) (h_1 : (x : String.Pos) → (cp : Nat) → motive 0 x cp)
   (h_2 : (utf16pos : Nat) → (utf8pos : String.Pos) → (cp : Nat) → motive utf16pos utf8pos cp) (x✝³ : String.Pos)
   (cp : Nat) (heq_1 : x✝ = 0) (heq_2 : x✝¹ = x✝³) (heq_3 : x✝² = cp) :
@@ -110,7 +110,7 @@ info: utf16PosToCodepointPosFromAux.match_1.gen_eq_1.{u_1} (motive : Nat → Str
     (h_1 x✝³ cp)
 -/
 #guard_msgs in
-#check utf16PosToCodepointPosFromAux.match_1.gen_eq_1
+#check utf16PosToCodepointPosFromAux.match_1.congr_eq_1
 
 opaque some_expr : Option Nat
 def wrongEq (m? : Option Nat) (h : some_expr = m?)
@@ -119,7 +119,7 @@ def wrongEq (m? : Option Nat) (h : some_expr = m?)
   | some m?, _ => exact true
 
 /--
-info: wrongEq.match_1.gen_eq_1.{u_1} (motive : (m? : Option Nat) → 0 < m?.getD 0 → some_expr = m? → Sort u_1)
+info: wrongEq.match_1.congr_eq_1.{u_1} (motive : (m? : Option Nat) → 0 < m?.getD 0 → some_expr = m? → Sort u_1)
   (m?✝ : Option Nat) (w✝ : 0 < m?✝.getD 0) (h : some_expr = m?✝)
   (h_1 : (m? : Nat) → (x : 0 < (some m?).getD 0) → (h : some_expr = some m?) → motive (some m?) x h) (m? : Nat)
   (x✝ : 0 < (some m?).getD 0) (h✝ : some_expr = some m?) (heq_1 : m?✝ = some m?) (heq_2 : HEq w✝ x✝)
@@ -129,7 +129,7 @@ info: wrongEq.match_1.gen_eq_1.{u_1} (motive : (m? : Option Nat) → 0 < m?.getD
     | some m?, x, h => h_1 m? x h)
     (h_1 m? x✝ h✝)
 -/
-#guard_msgs in #check wrongEq.match_1.gen_eq_1
+#guard_msgs in #check wrongEq.match_1.congr_eq_1
 
 set_option linter.unusedVariables false in
 noncomputable def myNamedPatternTest (x : List Bool) : Bool :=
@@ -138,7 +138,7 @@ noncomputable def myNamedPatternTest (x : List Bool) : Bool :=
   | x' => true
 
 /--
-info: myNamedPatternTest.match_1.gen_eq_1.{u_1} (motive : List Bool → Sort u_1) (x✝ : List Bool)
+info: myNamedPatternTest.match_1.congr_eq_1.{u_1} (motive : List Bool → Sort u_1) (x✝ : List Bool)
   (h_1 : (x' : List Bool) → (x : Bool) → (xs : List Bool) → x' = x :: xs → x✝ = x :: xs → motive (x :: xs))
   (h_2 : (x' : List Bool) → x✝ = x' → motive x') (x : Bool) (xs : List Bool) (heq_1 : x✝ = x :: xs) :
   HEq
@@ -148,15 +148,16 @@ info: myNamedPatternTest.match_1.gen_eq_1.{u_1} (motive : List Bool → Sort u_1
     (h_1 (x :: xs) x xs ⋯ heq_1)
 -/
 #guard_msgs in
-#check myNamedPatternTest.match_1.gen_eq_1
+#check myNamedPatternTest.match_1.congr_eq_1
 
+set_option linter.unusedVariables false in
 def testMe (n : Nat) : Bool :=
   match _ : n - 2 with
   | 0 => true
   | m => false
 
 /--
-info: testMe.match_1.gen_eq_2.{u_1} (motive : Nat → Sort u_1) (x✝ : Nat) (h_1 : x✝ = 0 → motive 0)
+info: testMe.match_1.congr_eq_2.{u_1} (motive : Nat → Sort u_1) (x✝ : Nat) (h_1 : x✝ = 0 → motive 0)
   (h_2 : (m : Nat) → x✝ = m → motive m) (m : Nat) (heq_1 : x✝ = m) :
   (m = 0 → False) →
     HEq
@@ -166,9 +167,9 @@ info: testMe.match_1.gen_eq_2.{u_1} (motive : Nat → Sort u_1) (x✝ : Nat) (h_
       (h_2 m heq_1)
 -/
 #guard_msgs in
-#check testMe.match_1.gen_eq_2
+#check testMe.match_1.congr_eq_2
 
--- JFR: Code to check if all matchers with equations also have generalize equations
+-- JFR: Code to check if all matchers with equations also have congruence equations
 /-
 open Lean Meta in
 run_meta do
@@ -184,7 +185,7 @@ run_meta do
           pure ()
         if ok then
           try
-            let _ ← Lean.Meta.Match.Match.genGeneralizedMatchEqns k
+            let _ ← Lean.Meta.Match.Match.gendMatchCongrEqns k
           catch e =>
             logError m!"failed to generate equations for {k} in {.ofConstName k.getPrefix}\n{indentD e.toMessageData}"
 -/
